cedar-lean/Cedar/Thm/TPE.lean
@@ -63,13 +63,13 @@ theorem reauthorize_is_sound
   intro hv h_auth
 
   simp only [TPE.isAuthorized] at h_auth
-  cases h_auth₁ : List.mapM (λ p => ResidualPolicy.mk p.id p.effect <$> evaluatePolicy schema p preq pes) policies <;> simp [h_auth₁] at h_auth
-  rename_i residuals
-  subst h_auth
+  cases h_auth₁ : isAuthorized.evaluatePolicies schema policies preq pes <;>
+    simp [h_auth₁] at h_auth
+  rw [← h_auth]
 
-  rw [List.mapM_ok_iff_forall₂] at h_auth₁
-  have equiv_satisfied := reauthorize_satisfied_policies_equiv hv h_auth₁
-  have equiv_errors := reauthorize_error_policies_equiv hv h_auth₁
+  have h_equiv := evaluatePolicies_residuals_equiv hv h_auth₁
+  have equiv_satisfied := reauthorize_satisfied_policies_equiv h_equiv
+  have equiv_errors := reauthorize_error_policies_equiv h_equiv
   simp [TPE.isAuthorized.isAuthorizedFromResiduals, Response.reauthorize, Spec.isAuthorized,
         equiv_satisfied .forbid, equiv_satisfied .permit, equiv_errors]
 
@@ -92,51 +92,10 @@ theorem partial_authorize_decision_is_sound
 := by
   intro h₁ h₂
   simp only [TPE.isAuthorized] at h₁
-
-  cases h₃ : List.mapM (λ p => ResidualPolicy.mk p.id p.effect <$> evaluatePolicy schema p preq pes) policies <;>
+  cases h₃ : isAuthorized.evaluatePolicies schema policies preq pes <;>
     simp [h₃] at h₁
-  rename_i rps
-
-  rw [List.mapM_ok_iff_forall₂] at h₃
-  simp [isAuthorized.isAuthorizedFromResiduals] at h₁
-  split at h₁ <;>
-    simp only [← h₁, reduceCtorEq, false_implies]
-  all_goals
-    intro h₅
-    simp only [Option.some.injEq] at h₅
-    subst h₅
-  -- Deny (satisfied forbid exists)
-  · have hf : ¬ (isAuthorized.satisfiedPolicies .forbid rps).isEmpty := by grind
-    have h_forbid : HasSatisfiedEffect Effect.forbid req es policies :=
-      satisfied_effect_if_non_empty_satisfied_policies h₂ h₃ hf
-
-    apply forbid_trumps_permit
-    unfold IsExplicitlyForbidden
-    exact h_forbid
-
-  -- Deny (no satisfied permits)
-  · have hp₁ : (isAuthorized.satisfiedPolicies .permit rps).isEmpty := by grind
-    have hp₂ : (isAuthorized.residualPolicies .permit rps).isEmpty := by grind
-    have h_not_permit : ¬HasSatisfiedEffect Effect.permit req es policies :=
-      no_satisfied_effect_if_empty_satisfied_and_residual_policies h₂ h₃ hp₁ hp₂
-
-    apply default_deny
-    unfold IsExplicitlyPermitted
-    exact h_not_permit
-
-  -- Allow (satisfied permit exists, no satisfied/residual forbids)
-  · have hf₁ : (isAuthorized.satisfiedPolicies .forbid rps).isEmpty := by grind
-    have hf₂ : (isAuthorized.residualPolicies .forbid rps).isEmpty := by grind
-    have h_not_forbid : ¬HasSatisfiedEffect Effect.forbid req es policies :=
-      no_satisfied_effect_if_empty_satisfied_and_residual_policies h₂ h₃ hf₁ hf₂
-
-    have hp : ¬ (isAuthorized.satisfiedPolicies .permit rps).isEmpty := by grind
-    have h_permit : HasSatisfiedEffect Effect.permit req es policies :=
-      satisfied_effect_if_non_empty_satisfied_policies h₂ h₃ hp
-
-    apply (allowed_iff_explicitly_permitted_and_not_denied _ _ _).mp
-    unfold IsExplicitlyPermitted IsExplicitlyForbidden
-    exact .intro h_permit h_not_forbid
+  rw [← h₁]
+  exact residuals_decision_agrees (evaluatePolicies_residuals_equiv h₂ h₃)
 
 /-- Trivial composition of the first two soundness theorems directly relating
 the decision of partial authorization and subsequent re-authorization.-/
@@ -175,15 +134,12 @@ theorem partial_authorize_erroring_policies_is_sound
 := by
   intro h₁ h₂
   simp only [TPE.isAuthorized] at h₁
-
-  cases h₃ : List.mapM (λ p => ResidualPolicy.mk p.id p.effect <$> evaluatePolicy schema p preq pes) policies <;>
+  cases h₃ : isAuthorized.evaluatePolicies schema policies preq pes <;>
     simp [h₃] at h₁
-  rename_i rps
-  rw [List.mapM_ok_iff_forall₂] at h₃
-  subst response
-
-  have h_err_permit := partial_authorize_error_policies_is_sound .permit h₃ h₂
-  have h_err_forbid := partial_authorize_error_policies_is_sound .forbid h₃ h₂
+  subst h₁
+  have h_equiv := evaluatePolicies_residuals_equiv h₂ h₃
+  have h_err_permit := partial_authorize_error_policies_is_sound .permit h_equiv
+  have h_err_forbid := partial_authorize_error_policies_is_sound .forbid h_equiv
   rw [Set.union_subset]
   exact .intro h_err_forbid h_err_permit
 
@@ -209,36 +165,13 @@ theorem partial_authorize_allow_determining_policies_is_sound
     grind [Spec.isAuthorized]
   simp only [Spec.isAuthorized, h_allow', Bool.not_false, Bool.and_self, ↓reduceIte]
 
-  cases h₃ : List.mapM (λ p => ResidualPolicy.mk p.id p.effect <$> evaluatePolicy schema p preq pes) policies <;>
+  cases h₃ : isAuthorized.evaluatePolicies schema policies preq pes <;>
     simp [h₃] at h₁
-  rename_i rps
-  rw [List.mapM_ok_iff_forall₂] at h₃
-  subst response
-
-  simp [isAuthorized.isAuthorizedFromResiduals, isAuthorized.satisfiedPolicies,
-    satisfiedPolicies, satisfiedWithEffect, satisfied, Bool.and_eq_true,
-    decide_eq_true_eq, Set.subset_def, Set.mem_make, List.mem_filterMap,
-    ResidualPolicy.satisfiedWithEffect, ResidualPolicy.satisfied, Residual.isTrue,
-    Option.ite_none_right_eq_some, forall_exists_index, and_imp]
-  intro pid rp hrp heff hs hpid
-  split at hs <;> try contradiction
-
-  have ⟨p, hp₁, hp₂⟩ := List.forall₂_implies_all_right h₃ rp hrp
-  cases hp₃ : evaluatePolicy schema p preq pes <;>
-   simp only [hp₃, Except.map_error, Except.map_ok, reduceCtorEq, Except.ok.injEq] at hp₂
-
-  exists p
-  and_intros
-  · exact hp₁
-  · rw [←hp₂] at heff
-    exact heff
-  · rename_i ty hr r
-    replace hr : r = .val (.prim (.bool true)) ty := by grind
-    have ha := partial_evaluate_policy_is_sound hp₃ h₂
-    simp only [hr, Residual.evaluate] at ha
-    exact to_option_right_ok' ha
-  · rw [←hp₂] at hpid
-    exact hpid
+  subst h₁
+  have h_equiv := evaluatePolicies_residuals_equiv h₂ h₃
+  exact Set.subset_trans
+    (partial_authorize_satisfied_policies_is_sound .permit h_equiv)
+    (by simp [Set.subset_def])
 
 /-- If the result of concrete authorization is `deny`, then any permit policies
 satisfied after partial authorization cannot be determining policies.  -/
@@ -293,12 +226,11 @@ theorem partial_authorize_satisfied_forbid_is_determining
 := by
   intro h₁ h₂
   simp only [TPE.isAuthorized] at h₁
-
-  cases h₃ : List.mapM (λ p => ResidualPolicy.mk p.id p.effect <$> evaluatePolicy schema p preq pes) policies <;>
-    simp only [bind_pure_comp, h₃, Except.map_ok, Except.map_error, Except.ok.injEq, reduceCtorEq] at h₁
+  cases h₃ : isAuthorized.evaluatePolicies schema policies preq pes <;>
+    simp [h₃] at h₁
+  subst h₁
+  have h_equiv := evaluatePolicies_residuals_equiv h₂ h₃
   rename_i rps
-  rw [List.mapM_ok_iff_forall₂] at h₃
-  subst response
 
   simp only [isAuthorized.isAuthorizedFromResiduals, isAuthorized.satisfiedPolicies, Set.subset_def,
     Set.mem_make, List.mem_filterMap, ResidualPolicy.satisfiedWithEffect,
@@ -306,35 +238,24 @@ theorem partial_authorize_satisfied_forbid_is_determining
     Option.ite_none_right_eq_some, Option.some.injEq, forall_exists_index, and_imp]
   intro pid rp hrp heff hs hpid
   split at hs <;> try contradiction
+  rename_i hf₅
 
-  have ⟨p, hp₁, hp₂⟩ := List.forall₂_implies_all_right h₃ rp hrp
-  cases hp₃ : evaluatePolicy schema p preq pes <;>
-    simp only [hp₃, Except.map_error, Except.map_ok, reduceCtorEq, Except.ok.injEq] at hp₂
-  rename_i ty hr r
+  have ⟨p, hp₁, h_id, h_eff, h_eval⟩ := List.forall₂_implies_all_right h_equiv rp hrp
 
   have ha : Spec.evaluate p.toExpr req es = .ok (.prim (.bool true)) := by
-    replace hr : r = .val (.prim (.bool true)) ty := by grind
-    have ha := partial_evaluate_policy_is_sound hp₃ h₂
-    simp only [hr, Residual.evaluate] at ha
-    exact to_option_right_ok' ha
+    simp only [hf₅, Residual.evaluate] at h_eval
+    exact to_option_left_ok' h_eval
 
   suffices h : pid ∈ satisfiedPolicies Effect.forbid policies req es by
     have hd : IsExplicitlyForbidden req es policies := by
-      exists p
-      and_intros <;> grind [satisfied]
-    replace hd : (Spec.isAuthorized req es policies).decision = .deny :=
-      forbid_trumps_permit _ _ _ hd
+      exists p; and_intros <;> grind [satisfied]
+    replace hd := forbid_trumps_permit _ _ _ hd
     grind [Spec.isAuthorized]
 
   simp only [satisfiedPolicies, satisfiedWithEffect, satisfied, Bool.and_eq_true, beq_iff_eq,
     decide_eq_true_eq, Set.mem_make, List.mem_filterMap, Option.ite_none_right_eq_some,
     Option.some.injEq]
-  exists p
-  and_intros
-  · exact hp₁
-  · simpa [←hp₂] using heff
-  · exact ha
-  · simpa [←hp₂] using hpid
+  exact ⟨p, hp₁, ⟨h_eff ▸ heff, ha⟩, h_id ▸ hpid⟩
 
 /-- Like `partial_authorize_satisfied_permits_not_determining_if_deny` for
 `forbid` policies, but we can prove a stronger theorem because any satisfied
